- 三角函数
  - P14

- 极限
  - $$\lim C=C$$
  - $$\lim _{x \rightarrow x_{0}} x=x_{0}$$
  - $$\lim _{x \rightarrow \infty} \frac{1}{x}=0$$
  - $$\lim _{x \rightarrow 0} \frac{\sin x}{x}=1$$
  - $$\lim _{x \rightarrow 0} \frac{\tan x}{x}=1$$
  - $$\lim _{x \rightarrow 0} \frac{\arcsin x}{x}=1$$
  - $$\lim _{x \rightarrow \infty}\left(1+\frac{1}{x}\right)^{x}=e$$
  - $$\lim _{x \rightarrow \infty}\left(1+\frac{a}{x}\right)^{b x}=e^{a b}$$
  - $$\lim _{x \rightarrow \infty}\left(\frac{x+k}{x-2 k}\right)^{x}=\lim _{x \rightarrow \infty} \frac{\left(1+\frac{k}{x}\right)^{x}}{\left(1-\frac{2 k}{x}\right)^{x}}=\frac{e^{k}}{e^{-2 k}}=e^{3 k}$$


- 等阶无穷小代换
  - $$\sin \mathrm{x} \sim \mathrm{x}$$
  - $$\tan \sim \mathrm{x}$$
  - $$\arctan \mathrm{x} \sim \mathrm{x}$$
  - $$\arcsin \mathrm{x} \sim \mathrm{x}$$
  - $$1-\cos x \sim \frac{x^{2}}{2}$$
  - $$\ln (1+x) \sim x$$
  - $$e^{x}-1 \sim x$$
  - $$\sqrt{1+x}-1 \sim \frac{x}{2}$$

- 导数
  - $$y=C \sim y^{\prime}=0$$
  - $$y=n^{x} \sim y^{\prime}=n^{x} \ln n$$
  - $$y=\log _{a} x \sim y^{\prime}=\frac{1}{x \ln a}$$
  - $$y=x^{n} \sim y^{\prime}=n x^{n-1}$$
  - $$y=\sqrt[n]{x} \sim y^{\prime}=\frac{x^{-\frac{n-1}{n}}}{n}$$
  - $$y=\frac{1}{x^{n}} y^{\prime}=-\frac{n}{x^{n+1}}$$
  - $$y=\sin x \sim y^{\prime}=\cos x$$
  - $$y=\cos x \sim y^{\prime}=-\sin x$$
  - $$y=\tan x \sim y^{\prime}=\frac{1}{\cos ^{2} x}=\sec ^{2} x$$
  - $$y=\cot x \sim y^{\prime}=\frac{-1}{\sin ^{2} x}=-\csc ^{2} x$$
  - $$y=\sec x \sim y^{\prime}=\sec x \tan x$$
  - $$y=\csc x \sim y^{\prime}=-\csc x \cot x$$
  - $$y=\arcsin x \sim y^{\prime}=\frac{1}{\sqrt{1-x^{2}}}$$
  - $$y=\arccos x \sim y^{\prime}=-\frac{1}{\sqrt{1-x^{2}}}$$
  - $$y=\arctan x \sim y^{\prime}=\frac{1}{1+x^{2}}$$
  - $$y=\operatorname{arccot} x \sim y^{\prime}=-\frac{1}{1+x^{2}}$$
  - $$y=\sinh x \sim y^{\prime}=\cosh x(双曲函数)$$

- 导数四则运算法则
  - $$(\mathrm{u} \pm \mathrm{v})^{\prime}=\mathrm{u}^{\prime} \pm \mathrm{v}^{\prime}$$
  - $$(u \cdot v)^{\prime}=u^{\prime} \cdot v+u \cdot v^{\prime}$$
  - $$(\mathrm{cu})^{\prime}=\mathrm{c} \cdot \mathrm{u}^{\prime}$$
  - $$\left(\frac{u}{v}\right)^{\prime}=\frac{u ! v-u \cdot v^{\prime}}{v^{2}}(v \neq 0)$$
  - $$\left(\frac{1}{v}\right)^{\prime}=-\frac{1}{v^{2}} \cdot v^{\prime}(v \neq 0)$$
  - $$(\mathrm{u} \cdot \mathrm{v} \cdot \mathrm{w})^{\prime}=\mathrm{u}^{\prime} \cdot \mathrm{v} \cdot \mathrm{w}+\mathrm{u} \cdot \mathrm{v}^{\prime} \cdot \mathrm{w}+\mathrm{u} \cdot \mathrm{v} \cdot \mathrm{w}^{\prime}$$

- 洛必达法则
  - $$\lim _{x \rightarrow a} \frac{f(x)}{g(x)}=\lim _{x \rightarrow a} \frac{f^{\prime}(x)}{g^{\prime}(x)}=A$$
